some errors yet

dafny_verification/donations.dfy
@@ -1,19 +1,18 @@
 class Donations{
    
-    var donor_id_list: array<int> := new int[150];
+    var donor_id_list: array<int>;
     
-    var blood_type_list: array<string> := new string[0];
+    var blood_type_list: array<string>;
 
-    var btypes: array<string> := new string[8];
-    btypes[0], btypes[1], btypes[2], btypes[3], btypes[4], btypes[5], btypes[6], btypes[7]:= "A+", "A-", "B+", "B-", "O+", "O-", "AB+", "AB-";
+    var btypes: array<string>;
 
-    var abnormalities: array<bool> := new bool[0];
+    var abnormalities: array<bool>;
 
-    var blood_amount: array<int> := new int[0];
+    var blood_amount: array<int>;
 
-    var added_to_bank: array<bool> := new bool[0];
+    var added_to_bank: array<bool>;
 
-    method IndexArray (donor_id_list: array<int>)
+ /*   method IndexArray (donor_id_list: array<int>)
     modifies donor_id_list
     ensures donor_id_list.Length <= 150
     ensures forall j::0<=j<donor_id_list.Length ==> donor_id_list[j]==j+1;
@@ -27,64 +26,63 @@ class Donations{
             i:=i+1;
         }
     }
-
+ */
 
     predicate Valid()
     reads this{
-        /*class invariant goes here, possibly about donor_ids, as other class   variables all change without conditions*/ 
-        forall i :: i in donor_id ==> donor_id_list[i]<=150;
+        forall i ::0<=i<150 ==> donor_id_list[i]<=150
     }    
 
-    predicate valid_blood_type(str: string)
+    predicate validate_blood_type(str: string)
     reads this{
-        i:=0;
-        while i< btypes.Length
-        invariant 0 <= i< btypes.Length
-        invariant forall k::0<=k<i ==> btypes[k] != str
-        {
-             if btypes[i] == str
-                 {return true;} 
-             else 
-                 {return false;}
-        }
+        exists i::0<=i<btypes.Length && btypes[i]==str
     }
 
     predicate validate_donor_id(id: int)
     reads this
     {
-        i:=0;
-        while i< donor_id_list.Length
-        invariant 0 <= i< donor_id_list.Length
-        invariant forall k::0<=k<i ==> donor_id_list[k] != id
-        {
-             if donor_id_list[i] == id
-                 {return true;} 
-             else 
-                 {return false;}
-        }
+        exists i::0<=i<donor_id_list.Length && donor_id_list[i]==id
     }
 
     predicate validate_blood_amount(amount: int)
     reads this{
-        if (amount>450&&amount<550) {return true;} else {return false;};
+        amount > 450 && amount < 550
     }
 
     constructor()
     modifies this
     ensures Valid()
+    ensures donor_id_list.Length <= 150
+    ensures forall j::0<=j<donor_id_list.Length ==> donor_id_list[j]==j+1;
     {
-        //?
+        donor_id_list:= new int[150];
+
+        var i:=0;
+        while i<donor_id_list.Length
+        invariant 0<=i<donor_id_list.Length
+        invariant forall j::0<=j<i ==> donor_id_list[j]==j+1;
+        {
+            donor_id_list[i]:=i+1;
+            i:=i+1;
+        }
+
+        blood_type_list:= new string[0];
+        btypes := new string[8];
+        btypes[0], btypes[1], btypes[2], btypes[3], btypes[4], btypes[5], btypes[6], btypes[7]:= "A+", "A-", "B+", "B-", "O+", "O-", "AB+", "AB-";
+        abnormalities := new bool[0];
+        blood_amount := new int[0];
+        added_to_bank := new bool[0];
     }
 
-    method Accept_donation(b_type:string, abnormal:bool, amount:int)
+    method Accept_donation(id: int, b_type:string, abnormal:bool, amount:int)
     modifies blood_type_list
     modifies abnormalities
     modifies blood_amount
     modifies added_to_bank
     requires Valid()
-    requires validate_donor_id()
-    requires validate_blood_amount()
-    requires validate_blood_type()
+    requires validate_donor_id(id)
+    requires validate_blood_amount(amount)
+    requires validate_blood_type(b_type)
     ensures blood_type_list.Length == old(blood_type_list).Length +1
     ensures abnormalities.Length == old(abnormalities).Length +1
     ensures blood_amount.Length == old(blood_amount).Length +1
@@ -104,8 +102,6 @@ class Donations{
 
 method Main(){
     var donate:= new Donations();
-    donate.Accept_donation("A+", false, 500);
+    donate.Accept_donation(5, "A+", false, 500);
 }
-method Main(){
-//for testing by creating a new object of Donations class
-}
+
